src/spec/properties/TLS13.ConnectionState.ProtectedWireRecordAlignment.fst
@@ -511,6 +511,7 @@ let lemma_server_handshake_install_materials_agree_from_key_schedule
         | _, _ ->
           False) /\
         Seq.equal server_hs.hs_transcript client_hs.hs_transcript /\
+        negotiated_aead_alg server_hs == negotiated_aead_alg client_hs /\
         traffic_install_matches_key_schedule_for_role
           ServerEndpoint
           server_hs
@@ -540,13 +541,13 @@ let lemma_server_handshake_install_materials_agree_from_key_schedule
     Seq.lemma_eq_elim server_hs.hs_transcript client_hs.hs_transcript;
     assert (server_material ==
       traffic_key_material_for_secret
-        C.AEAD_CHACHA20_POLY1305
+        (negotiated_aead_alg server_hs)
         (K.server_handshake_traffic_secret
           server_secret
           (Tr.hash server_hs.hs_transcript)));
     assert (client_material ==
       traffic_key_material_for_secret
-        C.AEAD_CHACHA20_POLY1305
+        (negotiated_aead_alg client_hs)
         (K.server_handshake_traffic_secret
           client_secret
           (Tr.hash client_hs.hs_transcript)));
@@ -575,6 +576,8 @@ let lemma_server_handshake_write_client_handshake_read_install_aligned_from_key_
         Seq.equal
           server.model_handshake.hs_transcript
           client.model_handshake.hs_transcript /\
+        negotiated_aead_alg server.model_handshake ==
+          negotiated_aead_alg client.model_handshake /\
         traffic_install_matches_key_schedule_for_role
           ServerEndpoint
           server.model_handshake
@@ -728,6 +731,7 @@ let lemma_client_handshake_install_materials_agree_from_key_schedule
         | _, _ ->
           False) /\
         Seq.equal client_hs.hs_transcript server_hs.hs_transcript /\
+        negotiated_aead_alg client_hs == negotiated_aead_alg server_hs /\
         traffic_install_matches_key_schedule
           client_hs
           {
@@ -757,13 +761,13 @@ let lemma_client_handshake_install_materials_agree_from_key_schedule
     Seq.lemma_eq_elim client_hs.hs_transcript server_hs.hs_transcript;
     assert (client_material ==
       traffic_key_material_for_secret
-        C.AEAD_CHACHA20_POLY1305
+        (negotiated_aead_alg client_hs)
         (K.client_handshake_traffic_secret
           client_secret
           (Tr.hash client_hs.hs_transcript)));
     assert (server_material ==
       traffic_key_material_for_secret
-        C.AEAD_CHACHA20_POLY1305
+        (negotiated_aead_alg server_hs)
         (K.client_handshake_traffic_secret
           server_secret
           (Tr.hash server_hs.hs_transcript)));
@@ -792,6 +796,8 @@ let lemma_client_handshake_write_server_handshake_read_install_aligned_from_key_
         Seq.equal
           client.model_handshake.hs_transcript
           server.model_handshake.hs_transcript /\
+        negotiated_aead_alg client.model_handshake ==
+          negotiated_aead_alg server.model_handshake /\
         traffic_install_matches_key_schedule
           client.model_handshake
           {
